Common.lean
@@ -3,5 +3,8 @@ import Common.Map
 import Common.Mathlib
 import Common.Name
 import Common.Notation
-import Common.Syntax
+import Common.Term
+import Common.Term.Normal
+import Common.Term.Classify
+import Common.Context
 import Common.Util
