Common/Mathlib.lean
@@ -1,23 +1,22 @@
 
-import Mathlib.Tactic.Basic
-import Mathlib.Tactic.Cases
-import Mathlib.Tactic.CasesM
-import Mathlib.Tactic.Clear!
-import Mathlib.Tactic.ClearExcept
-import Mathlib.Tactic.Clear_
-import Mathlib.Tactic.Common
-import Mathlib.Tactic.Congr!
-import Mathlib.Tactic.Constructor
-import Mathlib.Tactic.Linarith
-import Mathlib.Tactic.Linarith.Datatypes
-import Mathlib.Tactic.Linarith.Elimination
-import Mathlib.Tactic.Linarith.Frontend
-import Mathlib.Tactic.Linarith.Lemmas
-import Mathlib.Tactic.Linarith.Parsing
-import Mathlib.Tactic.Linarith.Preprocessing
-import Mathlib.Tactic.Linarith.Verification
-import Mathlib.Tactic.Rename
-import Mathlib.Tactic.RenameBVar
-import Mathlib.Tactic.Replace
+-- import Mathlib.Tactic.Basic
+-- import Mathlib.Tactic.Cases
+-- import Mathlib.Tactic.CasesM
+-- import Mathlib.Tactic.ClearExcept
+-- import Mathlib.Tactic.Clear_
+-- import Mathlib.Tactic.Common
+-- import Mathlib.Tactic.Constructor
+-- import Mathlib.Tactic.Linarith
+-- import Mathlib.Tactic.Linarith.Datatypes
+-- import Mathlib.Tactic.Linarith.Elimination
+-- import Mathlib.Tactic.Linarith.Frontend
+-- import Mathlib.Tactic.Linarith.Lemmas
+-- import Mathlib.Tactic.Linarith.Parsing
+-- import Mathlib.Tactic.Linarith.Preprocessing
+-- import Mathlib.Tactic.Linarith.Verification
+-- import Mathlib.Tactic.Rename
+-- import Mathlib.Tactic.RenameBVar
+-- import Mathlib.Tactic.Replace
 
-import Std.Data.List.Lemmas
+-- import Mathlib.Data.List.Defs
+-- import Std.Data.List.Lemmas
