Common/Term.lean
@@ -1,0 +1,113 @@
+
+import Common.Mathlib
+
+inductive Mode where
+| free
+| erased
+| type
+deriving BEq
+
+notation "m0" => Mode.erased
+notation "mt" => Mode.type
+notation "mf" => Mode.free
+
+inductive Const : Type where
+| type : Const
+| kind : Const
+deriving BEq
+
+inductive CvTerm : Type where
+| sym : CvTerm -> CvTerm
+| ax : CvTerm
+| var : CvTerm
+| pi : CvTerm -> CvTerm -> CvTerm
+| lam_mt : CvTerm -> CvTerm -> CvTerm
+| lam_mf : CvTerm -> CvTerm
+| lam_eta : CvTerm -> CvTerm
+| lam_m0 : CvTerm -> CvTerm
+| app : CvTerm -> CvTerm -> CvTerm
+| app_beta : CvTerm -> CvTerm
+| app_m0 : CvTerm -> CvTerm
+| prod : CvTerm -> CvTerm -> CvTerm
+| pair : CvTerm -> CvTerm
+| fst : CvTerm -> CvTerm
+| snd : CvTerm -> CvTerm
+| eq : CvTerm -> CvTerm -> CvTerm -> CvTerm
+| refl : CvTerm -> CvTerm
+| subst : CvTerm -> CvTerm
+| conv : CvTerm -> CvTerm
+deriving BEq
+
+inductive Term : Type where
+| bound : Const -> Nat -> Term
+| none : Term
+| const : Const -> Term
+| lam : Mode -> Term -> Term -> Term
+| app : Mode -> Term -> Term -> Term
+| all : Mode -> Term -> Term -> Term
+| pair : Term -> Term -> Term -> Term
+| fst : Term -> Term
+| snd : Term -> Term
+| prod : Term -> Term -> Term
+| refl : Term -> Term
+| subst : Term -> Term -> Term
+| phi : Term -> Term -> Term -> Term
+| eq : Term -> Term -> Term -> Term
+| conv : Term -> Term -> CvTerm -> Term
+deriving BEq
+
+notation "★" => Term.const Const.type
+notation "□" => Term.const Const.kind
+
+instance : Inhabited Term where
+  default := Term.none
+
+namespace Term
+
+  -- templates
+  -- | i, bound k => sorry
+  -- | i, none => sorry
+  -- | i, type => sorry
+  -- | i, kind => sorry
+  -- | i, lam t1 t2 => sorry
+  -- | i, app t1 t2 => sorry
+  -- | i, all t1 t2 => sorry
+  -- | i, pair t1 t2 => sorry
+  -- | i, fst t => sorry
+  -- | i, snd t => sorry
+  -- | i, prod t1 t2 => sorry
+  -- | i, eq t1 t2 t3 => sorry
+  -- | i, int t1 t2 => sorry
+  -- case bound => sorry
+  -- case none => sorry
+  -- case type => sorry
+  -- case kind => sorry
+  -- case lam t1 t2 ih1 ih2 => sorry
+  -- case app t1 t2 ih1 ih2 => sorry
+  -- case all t1 t2 ih1 ih2 => sorry
+  -- case pair t1 t2 ih1 ih2 => sorry
+  -- case fst t ih => sorry
+  -- case snd t ih => sorry
+  -- case prod t1 t2 ih1 ih2 => sorry
+  -- case eq t1 t2 t3 ih1 ih2 ih3 => sorry
+  -- case int t1 t2 ih1 ih2 => sorry
+
+  @[simp]
+  def size : Term -> Nat
+  | bound _ _ => 0
+  | none => 0
+  | const _ => 0
+  | lam _ t1 t2 => size t1 + size t2 + 1
+  | app _ t1 t2 => size t1 + size t2 + 1
+  | all _ t1 t2 => size t1 + size t2 + 1
+  | pair t1 t2 t3 => size t1 + size t2 + size t3 + 1
+  | fst t => size t + 1
+  | snd t => size t + 1
+  | prod t1 t2 => size t1 + size t2 + 1
+  | refl t => size t + 1
+  | subst t1 t2 => size t1 + size t2 + 1
+  | phi t1 t2 t3 => size t1 + size t2 + size t3 + 1
+  | eq t1 t2 t3 => size t1 + size t2 + size t3 + 1
+  | conv t1 t2 _ => size t1 + size t2 + 1
+
+end Term
