Common/Term/Normal.lean
@@ -1,0 +1,33 @@
+
+import Common.Term
+
+namespace Term
+
+  mutual
+    inductive Neutral : Term -> Prop where
+    | bound : Neutral (.bound c k)
+    | app : Neutral f ->  Normal a -> Neutral (.app m f a)
+    | fst : Neutral t -> Neutral (.fst t)
+    | snd : Neutral t -> Neutral (.snd t)
+    | subst : Normal P -> Neutral e -> Neutral (.subst P e)
+    | phi :  Normal a ->  Normal b -> Neutral e -> Neutral (.phi a b e)
+    | conv :  Normal B ->  Neutral t -> Neutral (.conv B t c)
+
+    inductive Normal : Term -> Prop where
+    | bound : Normal (.bound c k)
+    | const : Normal (.const K)
+    | lam : Normal A -> Normal t -> Normal (.lam m A t)
+    | app : Neutral f -> Normal a -> Normal (.app m f a)
+    | all : Normal A -> Normal B -> Normal (.all m A B)
+    | pair : Normal T -> Normal t -> Normal s -> Normal (.pair T t s)
+    | fst : Neutral t -> Normal (.fst t)
+    | snd : Neutral t -> Normal (.snd t)
+    | prod : Normal A -> Normal B -> Normal (.prod A B)
+    | refl : Normal t -> Normal (.refl t)
+    | subst : Normal P -> Neutral e -> Normal (.subst P e)
+    | phi : Normal a -> Normal b -> Neutral e -> Normal (.phi a b e)
+    | eq : Normal A -> Normal a -> Normal b -> Normal (.eq A a b)
+    | conv : Normal B -> Normal t -> Normal (.conv B t c)
+  end
+
+end Term
