Common/Term/Substitution.lean
@@ -1,0 +1,388 @@
+import Common.Term
+
+namespace Term
+  def Ren : Type := Nat -> Nat
+
+  inductive SubstAction : Type where
+  | rename : Nat -> SubstAction
+  | replace : Term -> SubstAction
+
+  namespace SubstAction
+    def size : SubstAction -> Nat
+    | .rename _ => 0
+    | .replace t => Term.size t
+
+  end SubstAction
+
+  def Subst : Type := Nat -> SubstAction
+
+  @[simp] def I : Ren := λ n => n
+  @[simp] def S : Ren := λ n => n + 1
+  @[simp] def Sn (x : Nat) : Ren := λ n => n + x
+  @[simp] def Pn (x : Nat) : Ren := λ n => n - x
+
+  namespace Ren
+    def lift : Ren -> Ren
+    | _, 0 => 0
+    | σ, n + 1 => σ n + 1
+
+    @[simp]
+    def apply : Ren -> Term -> Term
+    | σ, bound c k => bound c (σ k)
+    | _, none => none
+    | _, const k => const k
+    | σ, lam m t1 t2 => lam m (apply σ t1) (apply (lift σ) t2)
+    | σ, app m t1 t2 => app m (apply σ t1) (apply σ t2)
+    | σ, all m t1 t2 => all m (apply σ t1) (apply (lift σ) t2)
+    | σ, pair t1 t2 t3 => pair (apply σ t1) (apply σ t2) (apply σ t3)
+    | σ, fst t => fst (apply σ t)
+    | σ, snd t => snd (apply σ t)
+    | σ, prod t1 t2 => prod (apply σ t1) (apply (lift σ) t2)
+    | σ, refl t => refl (apply σ t)
+    | σ, subst t1 t2 => subst (apply σ t1) (apply σ t2)
+    | σ, phi t1 t2 t3 => phi (apply σ t1) (apply σ t2) (apply σ t3)
+    | σ, eq t1 t2 t3 => eq (apply σ t1) (apply σ t2) (apply σ t3)
+    | σ, conv t1 t2 c => conv (apply σ t1) (apply σ t2) c
+  end Ren
+
+  namespace Subst
+    def from_ren : Ren -> Subst
+    | σ, n => .rename (σ n)
+
+    def cons : SubstAction -> Subst -> Subst
+    | t, _, 0 => t
+    | _, σ, n + 1 => σ n
+
+    def lift : Subst -> Subst
+    | _, 0 => .rename 0
+    | σ, n + 1 => match (σ n) with
+      | .replace t => .replace (Ren.apply S t)
+      | .rename k => .rename (S k)
+
+    @[simp]
+    def apply : Subst -> Term -> Term
+    | σ, bound c k =>
+      match σ k with
+      | .replace t => t
+      | .rename n => bound c n
+    | _, none => none
+    | _, const k => const k
+    | σ, lam m t1 t2 => lam m (apply σ t1) (apply (lift σ) t2)
+    | σ, app m t1 t2 => app m (apply σ t1) (apply σ t2)
+    | σ, all m t1 t2 => all m (apply σ t1) (apply (lift σ) t2)
+    | σ, pair t1 t2 t3 => pair (apply σ t1) (apply σ t2) (apply σ t3)
+    | σ, fst t => fst (apply σ t)
+    | σ, snd t => snd (apply σ t)
+    | σ, prod t1 t2 => prod (apply σ t1) (apply (lift σ) t2)
+    | σ, refl t => refl (apply σ t)
+    | σ, subst t1 t2 => subst (apply σ t1) (apply σ t2)
+    | σ, phi t1 t2 t3 => phi (apply σ t1) (apply σ t2) (apply σ t3)
+    | σ, eq t1 t2 t3 => eq (apply σ t1) (apply σ t2) (apply σ t3)
+    | σ, conv t1 t2 c => conv (apply σ t1) (apply σ t2) c
+
+    def compose : Subst -> Subst -> Subst
+    | σ, τ, n => match (σ n) with
+      | .replace t => .replace (apply τ t)
+      | .rename k => τ k
+
+    def beta : Term -> Term -> Term
+    | s, t => apply (cons (.replace t) (from_ren I)) s
+  end Subst
+
+  notation:100 "r#" σ:110 => Subst.from_ren σ
+  notation:70 t:70 "::" σ:70 => Subst.cons t σ
+  notation:100 "^" σ:110 => Subst.lift σ
+  notation:90 "[" σ "]" t:89 => Subst.apply σ t
+  notation:90 τ:90 " ⊙ " σ:91 => Subst.compose σ τ
+  notation:90 s:90 "β[" t "]" => Subst.beta s t
+
+  @[simp] theorem subst_from_ren_x : (r#r) x = .rename (r x) :=
+    by unfold Subst.from_ren; rfl
+
+  @[simp] theorem subst_cons_zero (σ : Subst) : (s :: σ) 0 = s :=
+    by unfold Subst.cons; rfl
+  @[simp] theorem subst_cons_succ (σ : Subst) : (s :: σ) (n + 1) = σ n :=
+    by unfold Subst.cons; rfl
+
+  @[simp]
+  theorem subst_lift_is_ren_lift r : r#(Ren.lift r) = ^(r#r) := by {
+    funext; case _ x =>
+    cases x
+    case zero =>
+      unfold Subst.from_ren; unfold Ren.lift; simp
+      unfold Subst.lift; simp
+    case _ n =>
+      generalize lhsdef : (r#(Ren.lift r)) (n + 1) = lhs
+      generalize rhsdef : (^(r#r)) (n + 1) = rhs
+      unfold Subst.from_ren at lhsdef; simp at *
+      unfold Ren.lift at lhsdef; simp at *
+      unfold Subst.lift at rhsdef; simp at *
+      subst lhsdef; subst rhsdef; rfl
+  }
+
+  @[simp]
+  theorem subst_apply_is_ren_apply r t : Ren.apply r t = [r#r]t := by {
+    induction t generalizing r
+    any_goals (unfold Ren.apply; simp [*])
+  }
+
+  @[simp]
+  theorem subst_apply_I_is_id s : [r#I]s = s := by {
+    have lem : ^(r# I) = r# I := by {
+      funext
+      case _ x =>
+      cases x
+      case _ =>
+        unfold Subst.lift; simp
+      case _ x =>
+        unfold Subst.lift; simp
+    }
+    induction s
+    all_goals unfold Subst.apply
+    any_goals simp [*]
+  }
+
+  @[simp]
+  theorem subst_apply_twice_is_apply_compose s σ τ : [τ][σ]s = [τ ⊙ σ]s := by {
+    have lem1 τ : ^τ ⊙ r#S = r#S ⊙ τ := by {
+      funext
+      unfold Subst.compose; unfold Subst.from_ren; unfold S; simp
+      unfold Subst.lift; unfold S; simp
+      unfold Subst.from_ren; simp
+    }
+    have lem2 (σ:Subst) e : ^(σ ⊙ r#e) = ^σ ⊙ ^(r#e) := by {
+      funext; case _ n =>
+      cases n
+      . unfold Subst.from_ren; unfold Subst.compose; unfold Subst.lift; simp
+      case _ n =>
+        generalize lhsdef : (^σ ⊙ ^(r#e)) (n + 1) = lhs
+        unfold Subst.lift; simp
+        unfold Subst.compose; unfold Subst.from_ren; unfold S; simp
+        subst lhs; unfold Subst.compose; unfold Subst.lift; simp
+        unfold Subst.from_ren; unfold S; simp
+    }
+    have lem3 σ e s : [σ][r#e]s = [σ ⊙ r#e]s := by {
+      induction s generalizing σ e
+      any_goals simp [*]
+      case bound => unfold Subst.compose; simp
+      case lam _ _ _ ih => rw [<-subst_lift_is_ren_lift, ih]
+      case all _ _ _ ih => rw [<-subst_lift_is_ren_lift, ih]
+      case prod _ _ _ ih => rw [<-subst_lift_is_ren_lift, ih]
+    }
+    have lem4 σ τ : σ ⊙ τ ⊙ r#S = σ ⊙ (τ ⊙ r#S) := by {
+      funext; case _ x =>
+      cases x
+      any_goals (unfold Subst.compose; unfold Subst.from_ren; unfold S; simp)
+    }
+    have lem5 r1 r2 τ : r#r1 ⊙ (r#r2 ⊙ τ) = r#r1 ⊙ r#r2 ⊙ τ := by {
+      funext; case _ x =>
+        unfold Subst.compose; simp
+        cases τ x <;> simp at *
+        case _ t =>
+          have lem : [fun x => SubstAction.rename (r1 (r2 x))]t = [r#r1 ⊙ r#r2]t := by {
+            unfold Subst.compose; simp
+          }
+          rw [lem, lem3]
+    }
+    have lem6 e τ : ^(r#e) ⊙ ^τ = ^(r#e ⊙ τ) := by {
+      funext; case _ n =>
+      cases n
+      . unfold Subst.compose; unfold Subst.lift; simp
+      case _ n =>
+        have lem : ((^(r#e) ⊙ ^τ) ⊙ r#S) n = (^(r#e ⊙ τ) ⊙ r#S) n := by {
+          rw [lem1, lem4, lem1]
+          rw [<-subst_lift_is_ren_lift, lem5]; simp
+          rw [lem1, lem5]
+        }
+        unfold Subst.compose at lem; unfold S at lem; unfold Subst.from_ren at lem
+        unfold Subst.compose; unfold Subst.from_ren
+        simp at lem; simp [*]
+    }
+    have lem7 τ e s : [r#e][τ]s = [r#e ⊙ τ]s := by {
+      induction s generalizing τ e
+      any_goals simp [*]
+      case bound k =>
+        unfold Subst.compose; simp
+        cases τ k <;> simp at *
+      case lam _ _ _ ih => rw [<-subst_lift_is_ren_lift, ih, <-lem6]; simp
+      case all _ _ _ ih => rw [<-subst_lift_is_ren_lift, ih, <-lem6]; simp
+      case prod _ _ _ ih => rw [<-subst_lift_is_ren_lift, ih, <-lem6]; simp
+    }
+    have lem8 σ τ : σ ⊙ (r#S ⊙ τ) = σ ⊙ r#S ⊙ τ := by {
+      funext; case _ x =>
+        unfold Subst.compose; simp
+        cases τ x <;> simp at *
+        rw [lem3]; unfold Subst.compose; simp
+    }
+    have lem9 σ τ : r#S ⊙ (σ ⊙ τ) = r#S ⊙ σ ⊙ τ := by {
+      funext; case _ x =>
+        unfold Subst.compose; simp
+        cases τ x <;> simp at *
+        rw [lem7]; unfold Subst.compose; simp
+    }
+    have lem10 σ τ : ^σ ⊙ ^τ = ^(σ ⊙ τ) := by {
+      funext; case _ x =>
+      cases x
+      case _ => unfold Subst.compose; unfold Subst.lift; simp
+      case _ n =>
+        have lem : ((^σ ⊙ ^τ) ⊙ r#S) n = (^(σ ⊙ τ) ⊙ r#S) n := by {
+          rw [lem1, lem4, lem1, lem8, lem1, lem9]
+        }
+        unfold Subst.compose at lem; unfold S at lem; unfold Subst.from_ren at lem
+        unfold Subst.compose
+        simp at lem; simp [*]
+    }
+    induction s generalizing τ σ
+    any_goals simp [*]
+    case bound k =>
+      unfold Subst.compose; simp
+      cases σ k <;> simp
+  }
+
+  @[simp] -- βst = s[t.I]
+  theorem subst_valid1 : s β[t] = [.replace t :: r#I]s := by unfold Subst.beta; simp
+
+  @[simp] -- 0[s.σ ] = s
+  theorem subst_valid2_replace
+    : [.replace s :: σ]bound c 0 = s
+  := by unfold Subst.cons; simp
+
+  @[simp] -- 0[s.σ ] = s
+  theorem subst_valid2_rename
+    : [.rename k :: σ]bound c 0 = bound c k
+  := by unfold Subst.cons; simp
+
+  @[simp] -- ⇑σ = 0.(σ ◦ S)
+  theorem subst_valid3 : ^σ = .rename 0 :: (r#S ⊙ σ) := by {
+    funext; case _ x =>
+      unfold Subst.lift; simp
+      unfold Subst.compose; simp
+      cases x
+      case _ => simp
+      case _ n => simp
+  }
+
+  @[simp] -- 0.S = I
+  theorem subst_valid4 : .rename 0 :: r#S = r#I := by {
+    funext; case _ x =>
+    cases x
+    case _ =>
+      unfold Subst.cons; unfold Subst.from_ren; simp
+    case _ n =>
+      unfold Subst.cons; unfold Subst.from_ren; simp
+  }
+
+  @[simp] -- σ ◦ I = σ
+  theorem subst_valid5 : σ ⊙ r#I = σ := by {
+    funext; case _ x =>
+    unfold Subst.compose; unfold Subst.from_ren; unfold I; simp
+  }
+
+  @[simp] -- I ◦ σ = σ
+  theorem subst_valid6 : r#I ⊙ σ = σ := by {
+    funext; case _ x =>
+    unfold Subst.compose; simp
+    cases x
+    all_goals (split; simp [*])
+    case _ _ _ e => rw [e]
+    case _ _ _ e => rw [e]
+  }
+
+  @[simp] -- (σ ◦ τ) ◦ μ = σ ◦ (τ ◦ μ)
+  theorem subst_valid7 : σ ⊙ (τ ⊙ μ) = σ ⊙ τ ⊙ μ := by {
+    funext; case _ x =>
+      unfold Subst.compose; simp
+      cases μ x <;> simp
+      . unfold Subst.compose; simp
+  }
+
+  @[simp] -- (s.σ ) ◦ τ = s[τ].(σ ◦ τ)
+  theorem subst_valid8_replace
+    : τ ⊙ (.replace s :: σ) = .replace ([τ]s) :: (τ ⊙ σ)
+  := by {
+    funext; case _ x =>
+    cases x
+    all_goals (unfold Subst.compose; unfold Subst.cons; simp)
+  }
+
+  @[simp] -- (s.σ ) ◦ τ = s[τ].(σ ◦ τ)
+  theorem subst_valid8_rename
+    : τ ⊙ (.rename s :: σ) = (τ s) :: (τ ⊙ σ)
+  := by {
+    funext; case _ x =>
+    cases x
+    all_goals (unfold Subst.compose; unfold Subst.cons; simp)
+  }
+
+  @[simp] -- S ◦ (s.σ ) = σ
+  theorem subst_valid9 : (s :: σ) ⊙ r#S = σ := by {
+    funext; case _ x =>
+    cases x
+    all_goals {
+      unfold Subst.compose; unfold Subst.cons; unfold Subst.from_ren
+      unfold S; simp
+    }
+  }
+
+  -- @[simp] -- 0[σ ].(S ◦ σ ) = σ
+  -- theorem subst_valid10 : .rename 0 :: r#S ⊙ σ = σ := by {
+  --   funext; case _ x =>
+  --   cases x
+  --   case _ => {
+  --     unfold Subst.cons; simp;
+  --     sorry
+  --   }
+  --   case _ n => {
+  --     unfold Subst.cons; simp; unfold Subst.compose; simp
+  --     unfold S; sorry
+  --   }
+  -- }
+
+  -- (βst)[σ ] = β(s[⇑σ ])(t[σ ])
+  theorem subst_beta_distr : [σ](s β[t]) = ([^σ]s) β[ [σ]t ] := by simp
+
+  -- s[σ ][S] = s[S][⇑σ ]
+  theorem subst_rw_ex1 : [r#S][σ]s = [^σ][r#S]s := by simp
+  -- -- s[⇑σ ][t.I] = s[t.σ ]
+  theorem subst_rw_ex2 : [t::r#I][^σ]s = [t::σ]s := by simp
+  -- s[⇑σ ][t[σ ].I] = s[t.I][σ ]
+  theorem subst_rw_ex3 : [(.replace ([σ]t))::r#I][^σ]s = [σ][.replace t::r#I]s := by simp
+
+  def mode_to_sort : Mode -> Const
+  | mt => .kind
+  | mf => .type
+  | m0 => .type
+
+  @[simp] theorem mt_to_sort : mode_to_sort mt = .kind := rfl
+  @[simp] theorem mf_to_sort : mode_to_sort mf = .type := rfl
+  @[simp] theorem m0_to_sort : mode_to_sort m0 = .type := rfl
+
+  def eta : Mode -> Term -> Term -> Term
+  | m, A, t => lam m A (app m ([r#S]t) (bound (mode_to_sort m) 0))
+
+  @[simp] theorem S_after_Pn : (r#S ⊙ r#(Pn n)) (n + k) = .rename (k + 1) := by {
+    cases n
+    case _ => unfold Subst.compose; simp
+    case _ n => unfold Subst.compose; simp; omega
+  }
+
+  @[simp] theorem S_after_Pn_1 : (r#S ⊙ r#(Pn 1)) 1 = .rename 1 := by {
+    unfold Subst.compose; simp
+  }
+
+  -- theorem subst_S_classifies_free : [r#S]s = s -> ∀ σ, [σ]s = s := by {
+  --   intro h σ
+  --   induction s generalizing σ
+  --   any_goals (simp at *; simp [*])
+  --   any_goals simp
+  --   case bound i => {
+  --     cases i <;> simp at *
+  --     all_goals (exfalso; unfold S at *; simp at h)
+  --   }
+  --   case lam t1 t2 ih1 ih2 => {
+  --     unfold Subst.cons at *; simp at *
+  --   }
+  --   case all => sorry
+  --   case int => sorry
+  -- }
+end Term
