Common/Util.lean
@@ -5,13 +5,13 @@ def contra {A B} : (A -> B) -> Not B -> Not A := by
   intros h1 h2 h3
   exact (h2 (h1 h3))
 
-lemma demorgan : ¬ (A ∨ B) -> ¬ A ∧ ¬ B := by {
+theorem demorgan : ¬ (A ∨ B) -> ¬ A ∧ ¬ B := by {
   intro h; apply And.intro _ _
   intro h2; apply h (Or.inl h2)
   intro h2; apply h (Or.inr h2)
 }
 
-lemma demorgan3 : ¬ (A ∨ B ∨ C) -> ¬ A ∧ ¬ B ∧ ¬ C := by {
+theorem demorgan3 : ¬ (A ∨ B ∨ C) -> ¬ A ∧ ¬ B ∧ ¬ C := by {
   intro h
   have lem := demorgan h
   cases lem; case _ h1 h2 =>
@@ -21,38 +21,34 @@ lemma demorgan3 : ¬ (A ∨ B ∨ C) -> ¬ A ∧ ¬ B ∧ ¬ C := by {
   apply And.intro h3 h4
 }
 
-lemma demorgan4 : ¬ (A ∨ B ∨ C ∨ D) -> ¬ A ∧ ¬ B ∧ ¬ C ∧ ¬ D := by {
-  intro h
-  have lem := demorgan3 h
-  casesm* _ ∧ _; case _ h1 h2 h3 =>
-  have lem2 := demorgan h3
-  cases lem2; case _ h4 h5 =>
-  apply And.intro h1 (And.intro h2 (And.intro h4 h5))
-}
+-- theorem demorgan4 : ¬ (A ∨ B ∨ C ∨ D) -> ¬ A ∧ ¬ B ∧ ¬ C ∧ ¬ D := by {
+--   intro h
+--   have lem := demorgan3 h
+--   casesm* _ ∧ _; case _ h1 h2 h3 =>
+--   have lem2 := demorgan h3
+--   cases lem2; case _ h4 h5 =>
+--   apply And.intro h1 (And.intro h2 (And.intro h4 h5))
+-- }
 
 def ne_sym : x ≠ y -> y ≠ x := by intro h1 h2; subst h2; contradiction
 
 def append_eq {a c : List α} {b d : α} : a ++ [b] = c ++ [d] -> a = c ∧ b = d := by {
   intro h
   induction a generalizing c
-  case nil => {
+  case nil =>
     rw [List.nil_append] at h
     cases c
-    case nil => {
+    case nil =>
       rw [List.nil_append] at h
       injection h with e1 e2; simp [*]
-    }
     case cons hd tl => injection h with e1 e2; simp at *
-  }
-  case cons hd tl ih => {
+  case cons hd tl ih =>
     cases c
     case nil => injection h with e1 e2; simp at *
-    case cons hd' tl' => {
+    case cons hd' tl' =>
       injection h with e1 e2; simp at *
       have lem := ih e2
       simp [*]
-    }
-  }
 }
 
 def pair_eq : (a, b) = (c, d) -> a = c ∧ b = d := by {
