WCCC/Proof/Basic.lean
@@ -1,0 +1,8 @@
+
+import Common
+import WCCC.Proof
+
+namespace WCCC
+
+
+end WCCC
