WCCC/Proof/Classify.lean
@@ -1,0 +1,78 @@
+
+import Common
+import WCCC.Proof
+
+namespace WCCC
+
+  theorem classify_proof
+    : Γ ⊢[m] t : A ->
+      (A = □) ∨ (Γ ⊢[mt] A : □) ∨ (Γ ⊢[mt] A : ★)
+  := by {
+    intro j
+    induction j
+    case ax =>
+      sorry
+    case var =>
+      sorry
+    case lam Γ A m K t B C j1 j2 j3 ih1 ih2 ih3 =>
+      cases m
+      case _ =>
+        simp at *; apply Or.inr
+        constructor
+        case h.K => exact K
+        all_goals simp [*]
+      case _ =>
+        simp at *; apply Or.inr
+        constructor
+        case h.K => exact K
+        all_goals simp [*]
+      case _ =>
+        simp at *; apply Or.inl
+        constructor
+        case h.K => exact K
+        all_goals simp [*]
+    case pi =>
+      sorry
+    case app Γ m1 f m2 A B a j1 j2 ih1 ih2 =>
+      cases m2
+      case _ =>
+        apply Or.inr; apply Or.inr
+        cases ih1
+        case _ ih1 => injection ih1
+        case _ ih1 =>
+          cases ih1
+          case _ ih1 => cases ih1
+          case _ ih1 =>
+            cases ih1
+            case _ K j3 j4 =>
+              simp at j4;
+              sorry
+      case _ =>
+        sorry
+      case _ =>
+        sorry
+    case prod =>
+      sorry
+    case pair =>
+      sorry
+    case fst =>
+      sorry
+    case snd =>
+      sorry
+    case eq =>
+      sorry
+    case refl =>
+      sorry
+    case subst =>
+      sorry
+    case conv =>
+      sorry
+  }
+
+  theorem term_classify_is_sound
+    : Γ ⊢[m] t : A -> (A = □ -> Term.classify t = .kind)
+      ∧ (Γ ⊢[mt] A : □ -> Term.classify t = .type)
+      ∧ (Γ ⊢[mt] A : ★ -> Term.classify t = .term)
+  := by sorry
+
+end WCCC
