lakefile.lean
@@ -1,7 +1,7 @@
 import Lake
 open Lake DSL
 
-require mathlib from git "https://github.com/leanprover-community/mathlib4"@"11980d2"
+require mathlib from git "https://github.com/leanprover-community/mathlib4"@"4ceb2ea935085e8145e880f754cef760063f16de"
 
 package «cedille2» {
   -- add package configuration options here
@@ -10,14 +10,11 @@ package «cedille2» {
 lean_lib Common where
   roots := #[`Common]
 
-lean_lib SystemFOmega where
-  roots := #[`SystemFOmega]
-
 lean_lib Cedille where
   roots := #[`Cedille]
 
-lean_lib Normalization where
-  roots := #[`Normalization]
+lean_lib WCCC where
+  roots := #[`WCCC]
 
 @[default_target]
 lean_exe «cedille» {
